NuSys.thy
@@ -1528,7 +1528,8 @@ lemma [\<nu>intro 70]: \<comment> \<open>OR search the later cells, if hasn't su
   by (rule cast_dual_intro_frame_R)
 
 lemma [\<nu>intro 30]:
-  "\<^bold>c\<^bold>a\<^bold>s\<^bold>t a \<R_arr_tail> x \<tycolon> T \<longmapsto>  a' \<R_arr_tail> x' \<tycolon> T' \<^bold>w\<^bold>i\<^bold>t\<^bold>h P \<^bold>d\<^bold>u\<^bold>a\<^bold>l a\<^sub>m \<R_arr_tail> x\<^sub>m \<tycolon> X\<^sub>m \<longmapsto> H\<^sub>m \<Longrightarrow>
+  "\<^bold>s\<^bold>i\<^bold>m\<^bold>p\<^bold>r\<^bold>e\<^bold>m a = a' \<Longrightarrow>
+   \<^bold>c\<^bold>a\<^bold>s\<^bold>t a \<R_arr_tail> x \<tycolon> T \<longmapsto>  a' \<R_arr_tail> x' \<tycolon> T' \<^bold>w\<^bold>i\<^bold>t\<^bold>h P \<^bold>d\<^bold>u\<^bold>a\<^bold>l a\<^sub>m \<R_arr_tail> x\<^sub>m \<tycolon> X\<^sub>m \<longmapsto> H\<^sub>m \<Longrightarrow>
    \<^bold>c\<^bold>a\<^bold>s\<^bold>t OBJ a \<R_arr_tail> x \<tycolon> T \<longmapsto> Nothing \<heavy_asterisk> OBJ a' \<R_arr_tail> x' \<tycolon> T' \<^bold>w\<^bold>i\<^bold>t\<^bold>h P \<^bold>d\<^bold>u\<^bold>a\<^bold>l Nothing \<heavy_asterisk> a\<^sub>m \<R_arr_tail> x\<^sub>m \<tycolon> X\<^sub>m \<longmapsto> OBJ H\<^sub>m"
   unfolding cast_def Separation_empty by (simp add: pair_forall nu_exps)
 
@@ -2333,7 +2334,7 @@ lemma Prog_Interface_proc: "TERM proc \<Longrightarrow> Prog_Interface name TYPE
   unfolding Prog_Interface_def ..
 
 lemma Prog_Interface_func:
-  "TERM f \<Longrightarrow> Prog_Interface name TYPE('a::lrep) TYPE('b::lrep) (func_wrap TYPE('a) TYPE('b) f)" 
+  "TERM f \<Longrightarrow> Prog_Interface name TYPE('a::lrep) TYPE('b::lrep) f" 
   unfolding Prog_Interface_def ..
 
 section \<open>Main implementation of the system\<close>
