ROOT2
@@ -1,8 +1,0 @@
-chapter NuSystem
-
-session NuSystem = Main +
-  description "
-    \<nu>-system.
-  "
-  theories
-    NuPrim
